
@prefix : <http://www.hbp.FIXME.org/hbp_activity_ontology/> .
@prefix owl: <http://www.w3.org/2002/07/owl#> .
@prefix dc: <http://purl.org/dc/elements/1.1/> .
@prefix rdf: <http://www.w3.org/1999/02/22-rdf-syntax-ns#> .
@prefix xml: <http://www.w3.org/XML/1998/namespace> .
@prefix xsd: <http://www.w3.org/2001/XMLSchema#> .
@prefix rdfs: <http://www.w3.org/2000/01/rdf-schema#> .
@prefix skos: <http://www.w3.org/2004/02/skos/core#> .
@prefix HBP_ACT: <http://www.hbp.FIXME.org/hbp_activity_ontology/> .
@base <http://www.hbp.FIXME.org/hbp_activity_ontology> .

<http://www.hbp.FIXME.org/hbp_activity_ontology> rdf:type owl:Ontology ;
         dc:title "Activity types vocabulary"@en;
         dc:subject "Activity types"@en;
         dc:creator "Silvia Jimenez <silvia.jimenez@epfl.ch>";
         owl:versionInfo "1.0";
         dc:contributor "Silvia Jimenez <silvia.jimenez@epfl.ch>".

#################################################################
#    Annotation properties
#################################################################

###  http://www.w3.org/2004/02/skos/core#definition
skos:definition rdf:type owl:AnnotationProperty .


#################################################################
#    Classes
#################################################################

###  http://www.hbp.FIXME.org/hbp_activity_ontology/0000001
HBP_ACT:0000001 rdf:type owl:Class ;
         rdfs:label "Activity"@en ;
         skos:definition "An activity is something that occurs over a period of time and acts upon or with entities; it may include consuming, processing, transforming, modifying, relocating, using, or generating entities"@en .


###  http://www.hbp.FIXME.org/hbp_activity_ontology/0000002
HBP_ACT:0000002 rdf:type owl:Class ;
         rdfs:subClassOf HBP_ACT:0000001 ;
         rdfs:label "Annotation"@en ;
         skos:definition "Action of adding an annotation to any entity in a PROVenance graph."@en .


###  http://www.hbp.FIXME.org/hbp_activity_ontology/0000004
HBP_ACT:0000004 rdf:type owl:Class ;
         rdfs:subClassOf HBP_ACT:0000001 ;
         rdfs:label "Computation"@en ;
         skos:definition "Computation is any type of calculation that follows a well-defined model understood and expressed as, for example, an algorithm, or a protocol."@en .


###  http://www.hbp.FIXME.org/hbp_activity_ontology/0000005
HBP_ACT:0000005 rdf:type owl:Class ;
         rdfs:subClassOf HBP_ACT:0000004 ,
                         HBP_ACT:0000002 ;
         rdfs:label "Classification"@en ;
         skos:definition "The action or process of classifying an observation using a computational process."@en .


###  http://www.hbp.FIXME.org/hbp_activity_ontology/0000006
HBP_ACT:0000006 rdf:type owl:Class ;
         rdfs:subClassOf HBP_ACT:0000001 ;
         rdfs:label "Experiment"@en .


###  http://www.hbp.FIXME.org/hbp_activity_ontology/0000007
HBP_ACT:0000007 rdf:type owl:Class ;
         rdfs:subClassOf HBP_ACT:0000001 ;
         rdfs:label "Revision"@en ;
         skos:definition "A change or a set of changes that correct or improve a previous version of a dataset."@en .


###  Generated by the OWL API (version 4.2.8.20170104-2310) https://github.com/owlcs/owlapi