@prefix : <http://www.hbp.FIXME.org/hbp_activity_ontology/> .
@prefix nsu: <http://www.FIXME.org/nsupper#> .
@prefix owl: <http://www.w3.org/2002/07/owl#> .
@prefix rdf: <http://www.w3.org/1999/02/22-rdf-syntax-ns#> .
@prefix xml: <http://www.w3.org/XML/1998/namespace> .
@prefix xsd: <http://www.w3.org/2001/XMLSchema#> .
@prefix rdfs: <http://www.w3.org/2000/01/rdf-schema#> .
@prefix skos: <http://www.w3.org/2004/02/skos/core#> .
@prefix HBP_ACT: <http://www.hbp.FIXME.org/hbp_activity_ontology/> .

<http://www.hbp.FIXME.org/hbp_activity_ontology> a owl:Ontology ;
	owl:imports <http://www.w3.org/2004/02/skos/core> .
# 
# 
# #################################################################
# #
# #    Classes
# #
# #################################################################
# 
# 
# http://www.hbp.FIXME.org/hbp_activity_ontology/0000001

HBP_ACT:0000001 a owl:Class ;
	rdfs:label "Activity"@en ;
	skos:definition "An activity is something that occurs over a period of time and acts upon or with entities; it may include consuming, processing, transforming, modifying, relocating, using, or generating entities"@en .
# 
# http://www.hbp.FIXME.org/hbp_activity_ontology/0000002

HBP_ACT:0000002 a owl:Class ;
	rdfs:subClassOf HBP_ACT:0000001 ;
	rdfs:label "Annotation"@en ;
	skos:definition "Action of adding an annotation to any entity in a PROVenance graph."@en .
# 
# http://www.hbp.FIXME.org/hbp_activity_ontology/0000004

HBP_ACT:0000004 a owl:Class ;
	rdfs:subClassOf HBP_ACT:0000001 ;
	rdfs:label "Computation"@en ;
	skos:definition "Computation is any type of calculation that follows a well-defined model understood and expressed as, for example, an algorithm, or a protocol."@en .
# 
# http://www.hbp.FIXME.org/hbp_activity_ontology/0000005

HBP_ACT:0000005 a owl:Class ;
	rdfs:subClassOf HBP_ACT:0000002 , HBP_ACT:0000004 ;
	rdfs:label "Classification"@en ;
	skos:definition "The action or process of classifying an observation using a computational process."@en .
# 
# http://www.hbp.FIXME.org/hbp_activity_ontology/0000006

HBP_ACT:0000006 a owl:Class ;
	rdfs:subClassOf HBP_ACT:0000001 ;
	rdfs:label "Experiment"@en .
# 
# http://www.hbp.FIXME.org/hbp_activity_ontology/0000007

HBP_ACT:0000007 a owl:Class ;
	rdfs:subClassOf HBP_ACT:0000001 ;
	rdfs:label "Revision"@en ;
	skos:definition "A change or a set of changes that correct or improve a previous version of a dataset."@en .
# 
# Generated by the OWL API (version 4.2.5.20160517-0735) https://github.com/owlcs/owlapi
