@prefix : <http://www.hbp.FIXME.org/hbp_brain_atlas_template_ontology/> .
@prefix obo: <http://purl.obolibrary.org/obo/> .
@prefix owl: <http://www.w3.org/2002/07/owl#> .
@prefix rdf: <http://www.w3.org/1999/02/22-rdf-syntax-ns#> .
@prefix xml: <http://www.w3.org/XML/1998/namespace> .
@prefix xsd: <http://www.w3.org/2001/XMLSchema#> .
@prefix rdfs: <http://www.w3.org/2000/01/rdf-schema#> .
@prefix skos: <http://www.w3.org/2004/02/skos/core#> .
@prefix HBP_BATT: <http://www.hbp.FIXME.org/hbp_brain_atlas_template_ontology/> .

<http://www.hbp.FIXME.org/hbp_brain_atlas_template_ontology> a owl:Ontology ;
	owl:imports <http://www.w3.org/2004/02/skos/core> .
# 
# 
# #################################################################
# #
# #    Classes
# #
# #################################################################
# 
# 
# http://www.hbp.FIXME.org/hbp_brain_atlas_template_ontology/0000000

HBP_BATT:0000000 a owl:Class ;
	rdfs:label "Brain atlas template"@en .
# 
# http://www.hbp.FIXME.org/hbp_brain_atlas_template_ontology/0000001

HBP_BATT:0000001 a owl:Class ;
	rdfs:subClassOf HBP_BATT:0000000 ;
	rdfs:label "Allen adult mouse brain reference atlas V2"@en ;
	skos:definition "Allen mouse common coordinate framework (CCF) version 2 released in 2011 consists of 860 structures were extracted and interpolated to create symetric 3D annotations, provided by the Allen Institute"@en .
# 
# http://www.hbp.FIXME.org/hbp_brain_atlas_template_ontology/0000002

HBP_BATT:0000002 a owl:Class ;
	rdfs:subClassOf HBP_BATT:0000000 ;
	rdfs:label "Allen adult mouse brain reference atlas V3"@en ;
	skos:definition "Allen mouse common coordinate framework (CCF) version 3 released in 2015 is based on a 3D 10um isotropic highly detailed population average of 1675 specimens, provided by the Allen Institute."@en .
# 
# http://www.hbp.FIXME.org/hbp_brain_atlas_template_ontology/0000003

HBP_BATT:0000003 a owl:Class ;
	rdfs:subClassOf HBP_BATT:0000000 ;
	rdfs:label "Waxholm Space rat brain atlas v.2.0"@en ;
	skos:definition "The rat brain atlas template consists of T2*-weighted anatomical MRI at 39 μm isotropic voxels and diffusion tensor imaging (DTI) volumes at 78 μm isotropic voxels resolution from an 80 day old male Sprague Dawley rat, provided by the University of Oslo."@en .
# 
# http://www.hbp.FIXME.org/hbp_brain_atlas_template_ontology/0000004

HBP_BATT:0000004 a owl:Class ;
	rdfs:subClassOf HBP_BATT:0000000 ;
	rdfs:label "BigBrain"@en ;
	skos:definition "High 20 microns resolution whole human brain volumetric data release 2015 based on January 2015, provided by Montreal Neurological Institute and Forschungszentrum Jülich GmbH."@en .
# 
# http://www.hbp.FIXME.org/hbp_brain_atlas_template_ontology/0000005

HBP_BATT:0000005 a owl:Class ;
	rdfs:subClassOf HBP_BATT:0000000 ;
	rdfs:label "MNI Colin 27"@en ;
	skos:definition "Atlas built from one individual scanned 27 times, the images are linearly registered to create an average with high SNR and structure definition. Not originnally intended but adopted by many groups as a stereotaxic template. Provided by the McConnell Brain Imaging Centre, Montreal Neurological Institute, McGill University."@en .
# 
# http://www.hbp.FIXME.org/hbp_brain_atlas_template_ontology/0000006

HBP_BATT:0000006 a owl:Class ;
	rdfs:subClassOf HBP_BATT:0000000 ;
	rdfs:label "Infant brain atlas"@en ;
	skos:definition "Infant template parecelled in 94 regions (47 on each hemisphere) from a7.1 week-old girl, provided by the Commissariat a l'énergie atomique et aux énergies alternatives (CEA)."@en .
# 
# http://www.hbp.FIXME.org/hbp_brain_atlas_template_ontology/0000007

HBP_BATT:0000007 a owl:Class ;
	rdfs:subClassOf HBP_BATT:0000000 ;
	rdfs:label "MNI ICBM 152 nonlinear 6th generation."@en ;
	skos:definition "This is a version of the ICBM Average Brain - an average of 152 T1-weighted MRI scans, linearly and non-linearly (6 iterations) transformed to form a symmetric model in Talairach space - that is specially adapted for use with the MNI Linear Registration Package (mni_autoreg). Provided by the McConnell Brain Imaging Centre, Montreal Neurological Institute, McGill University."@en .
# 
# http://www.hbp.FIXME.org/hbp_brain_atlas_template_ontology/0000008

HBP_BATT:0000008 a owl:Class ;
	rdfs:subClassOf HBP_BATT:0000000 ;
	rdfs:label "Riken Marmoset Atlas"@en ;
	skos:definition "Axial-free steric brain atlas, a brain from the common marmoset monkey (Callithrix jacchus; female; 2.3 years old; weighting 310 g). Provided by RIKEN Brain Science Institute, Japan."@en .
# 
# Generated by the OWL API (version 4.2.5.20160517-0735) https://github.com/owlcs/owlapi
